No despair here

Clap/Test/Compiler/Traverse/Foldlm.lean
@@ -1,3 +1,4 @@
+import Lean
 import Clap.Test.Compiler.Traverse.Prelude
 
 namespace ExampruSym
@@ -8,33 +9,80 @@ open Clap.Compiler
 
 opaque share : ℕ → Option ℕ
 
--- abbrev sigma (x : ℕ) : Option (ℕ) := do
---   let x2 ← share (x * x)
---   let x4 ← share (x2 * x2)
---   some (x4 * x)
+def sigma (x : ℕ) : Option (ℕ) := do
+  let x2 ← share (x * x)
+  let x4 ← share (x2 * x2)
+  some (x4 * x)
 
-abbrev sigma_unshared (x : ℕ) : Option (ℕ) := do
+def sigma_unshared (x : ℕ) : Option (ℕ) := do
   let x2 ← some (x + x)
   let x4 ← some (x2 + x2)
+  -- let x8 ← some (x4 + x4)
   some (x4 + x)
 
 def testFoldlM : Option ℕ := do
-  let xs ← (List.range 10).foldlM (fun state r ↦ do
+  let xs ← (List.range 8).foldlM (fun state r ↦ do
     let s0 ← sigma_unshared state[0]
     state.set 0 s0
     ) #v[0, 1, 2]
   let x ← xs[0]
   return x
 
+def eq_def := sigma_unshared.eq_def
+
 -- set_option trace.Clap.Compile.simp.consiliumMagnum true in
 -- set_option trace.Clap.Compile.simp.proc.vector_foldlM_stagger true in
 -- set_option Clap.traversalDbg true in
--- set_option trace.Clap.Compile.dbg true in
--- -- set_option pp.exprSizes true in
+set_option trace.Clap.Compile.dbg true in
 -- set_option trace.Clap.Compile.simp.proc.beta true in
 set_option maxRecDepth 100000 in
 set_option maxHeartbeats 0 in
-#eval runOptionNTestByName ``testFoldlM
+#eval runOptionNTestByName ``testFoldlM (extraPasses := mkMethods #[
+  (``eq_def, .Pre)
+] (atMostOnce := false))
+
+
+-- THE PLAN
+-- use sigma unshared - done
+-- write a simproc that takes a list of simprocs and checks whether it itself has been run once from the debug state - done
+-- attempts to run these simprocs only if it hasn't - done
+-- reset its log in the debug state at the end of each consiliumMagnum iteration - done
+-- rejoice - todo
+
+
+
+open Lean Meta Elab Tactic
+
+elab "sym_simp" "[" declNames:ident,* "]" : tactic => do
+  let rewrite ← Sym.mkSimprocFor (← declNames.getElems.mapM fun s => realizeGlobalConstNoOverload s.raw) Sym.Simp.dischargeSimpSelf
+  let methods : Sym.Simp.Methods := {
+    pre  := Sym.Simp.simpControl
+    post := Sym.Simp.evalGround >> rewrite
+  }
+  liftMetaTactic1 fun mvarId => Sym.SymM.run do
+    let mvarId ← Sym.preprocessMVar mvarId
+    (← Sym.simpGoal mvarId methods).toOption
+
+example : testFoldlM = sorry := by
+  sym_simp [
+    testFoldlM.eq_def,
+    sigma_unshared.eq_def,
+    bind_assoc,
+    Option.bind_eq_bind,
+    Option.bind_some,
+    List.range.eq_def,
+    List.range.loop.eq_def,
+    List.foldlM_cons,
+    Vector.getElem_mk,
+    List.getElem_toArray,
+    List.getElem_cons_zero,
+    Vector.set_mk,
+    List.set_toArray,
+    List.set_cons_zero,
+    List.foldlM_nil,
+    Option.pure_def,
+    Option.bind_fun_some
+  ]
 
 end NewTraversal
 
